same for llist

pulse/examples/steel/CQueue.LList.fst
@@ -19,16 +19,145 @@ let cllist_tail #a c =
 
 #push-options "--ide_id_info_off"
 
-// TODO: follow CQueue.Cell
-let cllist_full_cllist #_ #a c = sladmit ()
-let alloc_cllist_full = admit ()
+let cllist0_refine
+  (#a: Type0)
+  (c: cllist_ptrvalue a)
+  (_: t_of emp)
+: Tot prop
+= cllist_ptrvalue_is_null c == false
 
-let alloc_cllist
+// unfold
+let cllist0_rewrite
+  (#a: Type0)
+  (c: cllist_ptrvalue a)
+  (_: t_of (emp `vrefine` cllist0_refine c))
+: Tot (cllist_lvalue a)
+= c
+
+[@@ __steel_reduce__]
+let cllist0 (a: Type0) (c: cllist_lvalue a) : Tot vprop =
+  (vptr (cllist_head c) `star` vptr (cllist_tail c))
+
+// unfold
+let cllist_rewrite
+  (#a: Type0)
+  (c: cllist_ptrvalue a)
+  (x: dtuple2 (cllist_lvalue a) (vdep_payload (emp `vrefine` cllist0_refine c `vrewrite` cllist0_rewrite c) (cllist0 a)))
+: GTot (vllist a)
+= let p =
+    dsnd #(cllist_lvalue a) #(vdep_payload (emp `vrefine` cllist0_refine c `vrewrite` cllist0_rewrite c) (cllist0 a)) x
+  in
+  {
+    vllist_head = fst p;
+    vllist_tail = snd p;
+  }
+
+[@@ __steel_reduce__ ; __reduce__] // to avoid manual unfoldings through change_slprop
+let cllist1
+  (#a: Type0)
+  (c: cllist_ptrvalue a)
+: Tot vprop
+= emp `vrefine` cllist0_refine c `vrewrite` cllist0_rewrite c `vdep` cllist0 a `vrewrite` cllist_rewrite c
+
+let cllist_hp
+  #a c
+= hp_of (cllist1 c)
+
+let cllist_sel
+  #a c
+= sel_of (cllist1 c)
+
+let intro_cllist
+  #opened #a c
+=
+  intro_vrefine emp (cllist0_refine c);
+  intro_vrewrite (emp `vrefine` cllist0_refine c) (cllist0_rewrite c);
+  reveal_star (vptr (cllist_head c)) (vptr (cllist_tail c));
+  intro_vdep
+    (emp `vrefine` cllist0_refine c `vrewrite` cllist0_rewrite c)
+    (vptr (cllist_head c) `star` vptr (cllist_tail c))
+    (cllist0 a);
+  intro_vrewrite
+    (emp `vrefine` cllist0_refine c `vrewrite` cllist0_rewrite c `vdep` cllist0 a)
+    (cllist_rewrite c);
+  change_slprop_rel
+    (cllist1 c)
+    (cllist c)
+    (fun x y -> x == y)
+    (fun m ->
+      assert_norm (hp_of (cllist1 c) == cllist_hp c);
+      assert_norm (sel_of (cllist1 c) m === sel_of (cllist c) m)
+    )
+
+let elim_cllist_ghost
+  #opened #a c
+=
+  change_slprop_rel
+    (cllist c)
+    (cllist1 c)
+    (fun x y -> x == y)
+    (fun m ->
+      assert_norm (hp_of (cllist1 c) == cllist_hp c);
+      assert_norm (sel_of (cllist1 c) m === sel_of (cllist c) m)
+    );
+  elim_vrewrite
+    (emp `vrefine` cllist0_refine c `vrewrite` cllist0_rewrite c `vdep` cllist0 a)
+    (cllist_rewrite c);
+  let c' : Ghost.erased (cllist_lvalue a) = elim_vdep
+    (emp `vrefine` cllist0_refine c `vrewrite` cllist0_rewrite c)
+    (cllist0 a)
+  in
+  elim_vrewrite (emp `vrefine` cllist0_refine c) (cllist0_rewrite c);
+  elim_vrefine emp (cllist0_refine c);
+  change_equal_slprop
+    (cllist0 a c')
+    (vptr (cllist_head (Ghost.reveal c')) `star` vptr (cllist_tail (Ghost.reveal c')));
+  reveal_star (vptr (cllist_head (Ghost.reveal c'))) (vptr (cllist_tail (Ghost.reveal c')));
+  c'
+
+let elim_cllist
+  #opened #a c
+=
+  let c2 = elim_cllist_ghost c in
+  let c : cllist_lvalue a = c in
+  change_equal_slprop (vptr (cllist_head c2)) (vptr (cllist_head c));
+  change_equal_slprop (vptr (cllist_tail c2)) (vptr (cllist_tail c));
+  return c
+
+let cllist_not_null
+  #opened #a c
+=
+  let c1 = elim_cllist_ghost c in
+  let c2 : cllist_lvalue a = c in
+  change_equal_slprop (vptr (cllist_head c1)) (vptr (cllist_head c2));
+  change_equal_slprop (vptr (cllist_tail c1)) (vptr (cllist_tail c2));
+  intro_cllist c2;
+  change_equal_slprop (cllist c2) (cllist c);
+  ()
+
+let freeable _ = True
+
+let ralloc (#a:Type0) (x:a) : Steel (ref a)
+  emp (fun r -> vptr r)
+  (requires fun _ -> True)
+  (ensures fun _ r h1 -> h1 (vptr r) == x /\ not (is_null r))
+=
+  alloc x
+
+let alloc_llist
   #a head tail
 =
-  let rhead = alloc_pt head in
-  let rtail = alloc_pt tail in
-  let gres = Ghost.hide ({ vllist_head = head; vllist_tail = tail }) in
-  let res = ({ head = rhead; tail = rtail; all_or_none_null = (); }, gres) in
-  rewrite_slprop (pts_to rhead full_perm head `star` pts_to rtail full_perm tail) (cllist (fst res) full_perm (snd res)) (fun _ -> ());
+  let rhead = ralloc head in
+  let rtail = ralloc tail in
+  let res : cllist_lvalue a = ({ head = rhead; tail = rtail; all_or_none_null = () }) in
+  change_equal_slprop (vptr rhead) (vptr (cllist_head res));
+  change_equal_slprop (vptr rtail) (vptr (cllist_tail res));
+  intro_cllist res;
   return res
+
+let free_llist
+  #a c
+=
+  let c = elim_cllist c in
+  free (cllist_head c);
+  free (cllist_tail c)
